proof/Preservation.v
@@ -196,7 +196,7 @@ Proof.
   - ii. des. exploit CALL; eauto. i; des. esplits; eauto.
     { etrans; eauto. }
     ii. exploit K; eauto. i; des. esplits; eauto. etrans; eauto.
-    etrans; eauto. etrans; eauto. eapply Sound.le_spec; eauto. eapply Sound.greatest_adq; eauto.
+    etrans; eauto. etrans; eauto. eapply Sound.vle_spec; eauto. eapply Sound.greatest_adq; eauto.
   - ii; des. exploit RET; eauto. i; des. esplits; eauto.
     etrans; eauto.
 Qed.
@@ -209,7 +209,7 @@ Inductive local_preservation_strong_horizontal (sound_state: Sound.t -> ms.(stat
         (SKENV: Sound.skenv su_arg args.(Args.m) ms.(ModSem.skenv))
         (INIT: ms.(ModSem.initial_frame) args st_init)
       ,
-        exists su_init, (<<LE: Sound.le su_arg su_init>>) /\
+        exists su_init, (<<LE: Sound.hle su_arg su_init>>) /\
                         (<<SUST: sound_state su_init st_init>>)
                         /\ (<<MLE: su_init.(Sound.mle) args.(Args.m) st_init.(get_mem)>>))
     (STEP: forall
@@ -219,7 +219,7 @@ Inductive local_preservation_strong_horizontal (sound_state: Sound.t -> ms.(stat
         (STEP: Step ms st0 tr st1)
       ,
         (* <<SUST: sound_state su0 st1>> /\ <<MLE: su0.(Sound.mle) st0.(get_mem) st1.(get_mem)>>) *)
-        exists su1, <<LE: Sound.le su0 su1>> /\ <<SUST: sound_state su1 st1>> /\ <<MLE: su0.(Sound.mle) st0.(get_mem) st1.(get_mem)>>)
+        exists su1, <<LE: Sound.hle su0 su1>> /\ <<SUST: sound_state su1 st1>> /\ <<MLE: su0.(Sound.mle) st0.(get_mem) st1.(get_mem)>>)
     (CALL: forall
         su0 st0 args
         (SUST: sound_state su0 st0)
@@ -234,7 +234,7 @@ Inductive local_preservation_strong_horizontal (sound_state: Sound.t -> ms.(stat
           (* (<<ARGS: su_lifted.(Sound.args) args>>) /\ *)
           (<<K: forall
               su_ret retv st1
-              (LE: Sound.le su_gr su_ret)
+              (LE: Sound.hle su_gr su_ret)
               (RETV: su_ret.(Sound.retv) retv)
               (* retv st1 *)
               (* (RETV: su_gr.(Sound.retv) retv) *)
@@ -242,7 +242,7 @@ Inductive local_preservation_strong_horizontal (sound_state: Sound.t -> ms.(stat
               (AFTER: ms.(ModSem.after_external) st0 retv st1)
             ,
               exists su1,
-                <<LE: Sound.le su0 su1>> /\
+                <<LE: Sound.hle su0 su1>> /\
               (* (<<SUST: sound_state su0 args.(Args.m) st1>>)>>)) *)
               (* (<<SUST: sound_state su0 st1>> /\ <<MLE: su0.(Sound.mle) st0.(get_mem) st1.(get_mem)>>)>>)) *)
               (<<SUST: sound_state su1 st1>> /\ <<MLE: su0.(Sound.mle) retv.(Retv.m) st1.(get_mem)>>)>>))
@@ -251,7 +251,7 @@ Inductive local_preservation_strong_horizontal (sound_state: Sound.t -> ms.(stat
         (SUST: sound_state su0 st0)
         (FINAL: ms.(ModSem.final_frame) st0 retv)
       ,
-        exists su_ret, <<LE: Sound.le su0 su_ret>> /\
+        exists su_ret, <<LE: Sound.hle su0 su_ret>> /\
         <<RETV: su_ret.(Sound.retv) retv>> /\ <<MLE: su0.(Sound.mle) st0.(get_mem) retv.(Retv.m)>>)
 .
 
@@ -262,34 +262,34 @@ Theorem local_preservation_strong_horizontal_spec
     <<PRSV: local_preservation (fun su m_init st =>
                                   <<MLE: su.(Sound.mle) m_init st.(get_mem)>> /\
                                   exists su_h,
-                                    <<LE: Sound.le su su_h>> /\ sound_state su_h st)>>
+                                    <<LE: Sound.hle su su_h>> /\ sound_state su_h st)>>
 .
 Proof.
   inv PRSV.
   econs; eauto.
-  - ii. exploit INIT; eauto. i; des. esplits; eauto. eapply Sound.le_spec; eauto.
+  - ii. exploit INIT; eauto. i; des. esplits; eauto. eapply Sound.hle_spec; eauto.
   - ii. des. exploit STEP; eauto. i; des. esplits; try apply SUST; eauto.
     + etrans; eauto.
-      eapply Sound.le_spec; eauto.
+      eapply Sound.hle_spec; eauto.
     + etrans; eauto.
   - ii. des. exploit CALL; eauto. i; des.
     exploit Sound.get_greatest_le; eauto. intro GRH. des.
-    assert(LE1: Sound.le su_h su_gr).
+    assert(LE1: Sound.vle su_h su_gr).
     { eapply Sound.greatest_adq; eauto. }
     esplits; eauto.
     { etrans; eauto.
-      + eapply Sound.le_spec; eauto.
+      + eapply Sound.hle_spec; eauto.
     }
     ii. exploit K; eauto. i; des. esplits; try apply SUST; eauto.
     + etrans; eauto.
-      eapply Sound.le_spec; eauto.
+      eapply Sound.hle_spec; eauto.
       etrans; eauto.
       etrans; eauto.
-      eapply Sound.le_spec; eauto.
+      eapply Sound.vle_spec; eauto.
     + etrans; eauto.
   - ii; des. exploit RET; eauto. i; des. esplits; try apply RETV; eauto.
     + etrans; eauto.
-    + etrans; eauto. eapply Sound.le_spec; eauto.
+    + etrans; eauto. eapply Sound.hle_spec; eauto.
 Qed.
 
 Inductive local_preservation_strong_excl (sound_state: Sound.t -> ms.(state) -> Prop): Prop :=
@@ -332,7 +332,7 @@ Inductive local_preservation_strong_excl (sound_state: Sound.t -> ms.(state) -> 
           (<<GR: Sound.get_greatest su0 args su_gr>>) /\
           (<<K: forall
               su_ret retv st1
-              (LE: Sound.le su_gr su_ret)
+              (LE: Sound.hle su_gr su_ret)
               (RETV: su_ret.(Sound.retv) retv)
               (MLE: Sound.mle su_gr args.(Args.m) retv.(Retv.m))
               (AFTER: ms.(ModSem.after_external) st0 retv st1)
@@ -343,7 +343,7 @@ Inductive local_preservation_strong_excl (sound_state: Sound.t -> ms.(state) -> 
         (SUST: sound_state su0 st0)
         (FINAL: ms.(ModSem.final_frame) st0 retv)
       ,
-        exists su_ret, <<LE: Sound.le su0 su_ret>> /\
+        exists su_ret, <<LE: Sound.hle su0 su_ret>> /\
         <<RETV: su_ret.(Sound.retv) retv>> /\ <<MLE: su0.(Sound.mle) st0.(get_mem) retv.(Retv.m)>>)
 .
 
@@ -361,7 +361,7 @@ Proof.
     { etrans; eauto. }
     ii. exploit K; eauto. i; des. esplits; eauto. etrans; eauto.
     etrans; eauto. etrans; eauto.
-    { eapply Sound.le_spec; eauto. eapply Sound.greatest_adq; eauto. }
+    { eapply Sound.vle_spec; eauto. eapply Sound.greatest_adq; eauto. }
     eapply FOOTWEAK; eauto.
     eapply FOOTLE; eauto.
   - ii; des. exploit RET; eauto. i; des. esplits; eauto.
@@ -389,7 +389,7 @@ Inductive local_preservation_strong_horizontal_excl (sound_state: Sound.t -> ms.
         (SKENV: Sound.skenv su_arg args.(Args.m) ms.(ModSem.skenv))
         (INIT: ms.(ModSem.initial_frame) args st_init)
       ,
-        exists su_init, (<<LE: Sound.le su_arg su_init>>) /\
+        exists su_init, (<<LE: Sound.hle su_arg su_init>>) /\
                         (<<SUST: sound_state su_init st_init>>)
                         /\ (<<MLE: su_init.(Sound.mle) args.(Args.m) st_init.(get_mem)>>))
     (STEP: forall
@@ -399,7 +399,7 @@ Inductive local_preservation_strong_horizontal_excl (sound_state: Sound.t -> ms.
         (STEP: Step ms st0 tr st1)
       ,
         (* <<SUST: sound_state su0 st1>> /\ <<MLE: su0.(Sound.mle) st0.(get_mem) st1.(get_mem)>>) *)
-        exists su1, <<LE: Sound.le su0 su1>> /\ <<SUST: sound_state su1 st1>> /\ <<MLE: su0.(Sound.mle) st0.(get_mem) st1.(get_mem)>>)
+        exists su1, <<LE: Sound.hle su0 su1>> /\ <<SUST: sound_state su1 st1>> /\ <<MLE: su0.(Sound.mle) st0.(get_mem) st1.(get_mem)>>)
     (CALL: forall
         su0 st0 args
         (SUST: sound_state su0 st0)
@@ -414,7 +414,7 @@ Inductive local_preservation_strong_horizontal_excl (sound_state: Sound.t -> ms.
           (* (<<ARGS: su_lifted.(Sound.args) args>>) /\ *)
           (<<K: forall
               su_ret retv st1
-              (LE: Sound.le su_gr su_ret)
+              (LE: Sound.hle su_gr su_ret)
               (RETV: su_ret.(Sound.retv) retv)
               (* retv st1 *)
               (* (RETV: su_gr.(Sound.retv) retv) *)
@@ -422,7 +422,7 @@ Inductive local_preservation_strong_horizontal_excl (sound_state: Sound.t -> ms.
               (AFTER: ms.(ModSem.after_external) st0 retv st1)
             ,
               exists su1,
-                <<LE: Sound.le su0 su1>> /\
+                <<LE: Sound.hle su0 su1>> /\
               (* (<<SUST: sound_state su0 args.(Args.m) st1>>)>>)) *)
               (* (<<SUST: sound_state su0 st1>> /\ <<MLE: su0.(Sound.mle) st0.(get_mem) st1.(get_mem)>>)>>)) *)
               (<<SUST: sound_state su1 st1>> /\ <<MLE: (mle_excl st0) su0 retv.(Retv.m) st1.(get_mem)>>)>>))
@@ -431,7 +431,7 @@ Inductive local_preservation_strong_horizontal_excl (sound_state: Sound.t -> ms.
         (SUST: sound_state su0 st0)
         (FINAL: ms.(ModSem.final_frame) st0 retv)
       ,
-        exists su_ret, <<LE: Sound.le su0 su_ret>> /\
+        exists su_ret, <<LE: Sound.hle su0 su_ret>> /\
         <<RETV: su_ret.(Sound.retv) retv>> /\ <<MLE: su0.(Sound.mle) st0.(get_mem) retv.(Retv.m)>>)
 .
 
@@ -442,36 +442,36 @@ Theorem local_preservation_strong_horizontal_excl_spec
     <<PRSV: local_preservation (fun su m_init st =>
                                   <<MLE: su.(Sound.mle) m_init st.(get_mem)>> /\
                                   exists su_h,
-                                    <<LE: Sound.le su su_h>> /\ sound_state su_h st)>>
+                                    <<LE: Sound.hle su su_h>> /\ sound_state su_h st)>>
 .
 Proof.
   inv PRSV.
   econs; eauto.
-  - ii. exploit INIT; eauto. i; des. esplits; eauto. eapply Sound.le_spec; eauto.
+  - ii. exploit INIT; eauto. i; des. esplits; eauto. eapply Sound.hle_spec; eauto.
   - ii. des. exploit STEP; eauto. i; des. esplits; try apply SUST; eauto.
     + etrans; eauto.
-      eapply Sound.le_spec; eauto.
+      eapply Sound.hle_spec; eauto.
     + etrans; eauto.
   - ii. des. exploit CALL; eauto. i; des.
     exploit Sound.get_greatest_le; eauto. intro GRH. des.
-    assert(LE1: Sound.le su_h su_gr).
+    assert(LE1: Sound.vle su_h su_gr).
     { eapply Sound.greatest_adq; eauto. }
     esplits; eauto.
     { etrans; eauto.
-      + eapply Sound.le_spec; eauto.
+      + eapply Sound.hle_spec; eauto.
     }
     ii. exploit K; eauto. i; des. esplits; try apply SUST; eauto.
     + etrans; eauto.
-      eapply Sound.le_spec; eauto.
+      eapply Sound.hle_spec; eauto.
       etrans; eauto.
       etrans; eauto.
-      * eapply Sound.le_spec; eauto.
+      * eapply Sound.vle_spec; eauto.
       * eapply FOOTWEAK; eauto.
         eapply FOOTLE; eauto.
     + etrans; eauto.
   - ii; des. exploit RET; eauto. i; des. esplits; try apply RETV; eauto.
     + etrans; eauto.
-    + etrans; eauto. eapply Sound.le_spec; eauto.
+    + etrans; eauto. eapply Sound.hle_spec; eauto.
 Qed.
 
 End PRSV.
